\documentclass[12]{scrartcl}
\usepackage{amssymb,amsmath,gensymb,dsfont,calc,multicol,fullpage,nbaseprt}
\makeatletter
\newcommand\Aboxed[1]{
   \@Aboxed#1\ENDDNE}
\def\@Aboxed#1&#2\ENDDNE{%
   &
   \settowidth\@tempdima{$\displaystyle#1{}$}
   \setlength\@tempdima{\@tempdima+\fboxsep+\fboxrule}
   \kern-\@tempdima
   \boxed{#1#2}
}
\makeatother

\begin{document}

\title{Homework 1, Section 1.2: 2, 5, 9, 21, 29}
\author{Alex Gordon}
\date{\today}
\maketitle

\section*{Homework}
\subsection*{2. A)}
\begin{multicols}{2}
\begin{align*} 
a_n &= 5n - 2
\\a_{k - 1} &= 5(k - 1) - 2
\\ & = 5k - 5 - 2 \\
\Aboxed{&= 5k - 7}
\end{align*}
\begin{align*} 
\\a_n &= 5n - 2
\\ a_{k + 1} &= 5(k + 1) - 2
\\ & = 5k + 5 - 2 \\
\Aboxed{& = 5k +3 }
\end{align*}
\end{multicols}

\subsection*{2. B)}
\begin{multicols}{2}
\begin{align*} 
a_n &= 3n^2 + n
\\ a_{k - 1} &= 3(k - 1)^2 + (k - 1)
\\ &= 3(k - 1)(k - 1) + (k - 1) \\
\Aboxed{& = 3k^2 - 5k + 2 }
\end{align*}
\begin{align*} 
\\ a_n &= 3n^2 + n
\\ a_{k + 1} &= 3(k + 1)^2 + (k + 1)
\\ &= 3(k - 1)(k + 1) + (k + 1) \\
\Aboxed{&= 3k^2 + 7k + 4}
\end{align*}
\end{multicols}

\subsection*{2. C)}
\begin{multicols}{2}
\begin{align*} 
a_n &= 2n + 7
\\ a_{k - 1} &= 2(k - 1) + 7
\\ &= 2k - 2 + 7 \\
\Aboxed{&= 2k + 5}
\end{align*}
\begin{align*} 
\\ a_n &= 2n + 7
\\ a_{k + 1} &= 2(k + 1) + 7
\\ &= 2k + 2 + 7 \\
\Aboxed{&= 2a + 9}
\end{align*}
\end{multicols}

\subsection*{2. D)}
\begin{multicols}{2}
\begin{align*} 
a_n &= 3^n + 4
\\ a_{k - 1} &= 3^{k - 1} + 4 \\
\Aboxed{&= 3^{k - 1} + 4}
\end{align*}
\begin{align*} 
\\ a_n &= 3^n + 4
\\ a_{k + 1} &= 3^{k + 1} + 4 \\
\Aboxed{&= 3^{k + 1} + 4}
\end{align*}
\end{multicols}

\subsection*{2. E)}
\begin{multicols}{2}
\begin{align*} 
a_n &= n^{3n +1} - 1 
\\ a_{k - 1} &= n^{3(k - 1) +1} - 1 
\\ &=  2^{3k - 3 +1} - 1\\
\Aboxed{&= 2^{3k - 2} - 1}
\end{align*}
\begin{align*} 
\\ a_n &= n^{3n +1} - 1 
\\ a_{k + 1} &= n^{3(k + 1) +1} - 1 
\\ &= n^{3k + 3 +1} - 1 \\
\Aboxed{&= 2^{3k + 4} - 1}
\end{align*}
\end{multicols}

\subsection*{2. F)}
\begin{multicols}{2}
\begin{align*} 
a_n &= \frac{n(2n - 1)(n + 2)}{6}
\\ a_{k - 1} &= \frac{k - 1(2(k - 1) - 1)((k - 1) + 2)}{6}
\\ &=  \frac{k - 1(2k - 2 - 1)(k +2)}{6}\\
\Aboxed{&= \frac{-2k^2-2k-3}{6}}
\end{align*}
\begin{align*} 
\\a_n &= \frac{n(2n - 1)(n + 2)}{6}
\\ a_{k + 1} &= \frac{k + 1(2(k + 1) - 1)(k + 1 + 2)}{6}
\\ &= \frac{k + 1(2k + 2) - 1)(k + 3)}{6}\\
\Aboxed{&= \frac{2k^2 +8k +3}{6}}
\end{align*}
\end{multicols}

\subsection*{5. A)}
 2, 4, 6, 8, 10 
\\ The pattern here is fairly obvious. It works out to \boxed{2n}.
\subsection*{5. B)}
1, 7, 13, 19, 25
\\There are a few answers to this pattern, however, the easiest one that I could find through experimenting is \boxed{6n - 5}
\subsection*{5. C)}
2, 5, 11, 23, 47
\\The pattern for this was a little harder to figure out. So to figure it out, I used the differences method. The differences are 3, 6, 12, 24. 
\subsection*{5. D)}
2, 4, 16, 256, 65536
\\$2^{2^n}$
\subsection*{9. A)}
5, 11, 18, 26, 35
\\$a_n$ = $\frac{1}{2}$
\subsection*{9. B)}
1, 4, 9, 16, 25
$a_n = n^2$
\subsection*{9. C)}
-3, 5, 17, 33, 53
$a_n = 2n(n + 1) -7$
\subsection*{21. A)}
\begin{align*} 
\sum\limits_{k=1}^7 &= 3k 
\\ \sum\limits_{k=1}^7 &= 3(1 + 2 + 3 + 4 + 5 + 6 +7) \\
\Aboxed{\sum\limits_{k=1}^7 &= 84}
\end{align*}
\subsection*{21. B)}
\begin{align*} 
\sum\limits_{k=1}^3 &= 3k
\\ \sum\limits_{k=1}^3 &= 3(1 + 2 + 3) \\
\Aboxed{\sum\limits_{k=1}^3 &= 42}
\end{align*}
\subsection*{21. C)}
\begin{align*} 
\sum\limits_{k=1}^9 &= 4 
\\ \sum\limits_{k=1}^9 &= 4(9) \\
\Aboxed{\sum\limits_{k=1}^9 &= 36}
\end{align*}
\subsection*{21. D)}
\begin{align*} 
\sum\limits_{k=0}^4 &= \frac{1}{2^k} \\
\Aboxed{\sum\limits_{k=0}^4 &= \frac{31}{16}}
\end{align*}
\subsection*{21. E)}
\begin{align*} 
\sum\limits_{k=-1}^3 &= 3- 2k\\
\Aboxed{\sum\limits_{k=-1}^3 &= 5}
\end{align*}
\subsection*{29. A)}
\begin{align*} 
\\a_3 &= A + ABBA + BA\\
\Aboxed{&= ABBABA}
\end{align*}
\begin{align*} 
\\a_4 &= A + a_{4-1} + BA \\
\Aboxed{&= AAABBABABA}
\end{align*}
\begin{align*} 
\\a_5 &= A + a_{5-1} + BA \\
\Aboxed{&= AAAABBABABABA}
\end{align*}
\begin{align*} 
\\a_6 &= A + a_{6-1} + BA \\
\Aboxed{&= AAAAABBABABABABA}
\end{align*}
\end{document}