\documentclass[12]{scrartcl}
\usepackage{amssymb,amsmath,gensymb,dsfont,calc,multicol,fullpage}
\makeatletter
\newcommand\Aboxed[1]{
   \@Aboxed#1\ENDDNE}
\def\@Aboxed#1&#2\ENDDNE{%
   &
   \settowidth\@tempdima{$\displaystyle#1{}$}
   \setlength\@tempdima{\@tempdima+\fboxsep+\fboxrule}
   \kern-\@tempdima
   \boxed{#1#2}
}
\makeatother

\begin{document}

\title{Homework 11, Section 2.2; 7, 10, 12, 14, 15, 18}
\author{Alex Gordon}
\date{\today}
\maketitle
\section*{Homework}
\subsection*{7. A)}
$A^-1b_1 = \begin{bmatrix} -9 \\ 4   \end{bmatrix}$
$A^-1b_2 = \begin{bmatrix} 11 \\ -5   \end{bmatrix}$
$A^-1b_3 = \begin{bmatrix} 6 \\ -2   \end{bmatrix}$
$A^-1b_4 = \begin{bmatrix} 13 \\ -5   \end{bmatrix}$
\subsection*{7. B)}
The solutions are the same as in part A. 
$A^-1b_1 = \begin{bmatrix} -9 \\ 4   \end{bmatrix}$
$A^-1b_2 = \begin{bmatrix} 11 \\ -5   \end{bmatrix}$
$A^-1b_3 = \begin{bmatrix} 6 \\ -2   \end{bmatrix}$
$A^-1b_4 = \begin{bmatrix} 13 \\ -5   \end{bmatrix}$

\subsection*{10. A)}
False. The product matrix is invertible, but the product of inverses should be in the reverse order. 
\subsection*{10. B)}
True, theorem 6a.
\subsection*{10. C)}
True, by theorem 4. 
\subsection*{10. D)}
True, by theorem 7. 
\subsection*{10. E)}
False, The theorem is not correct. 
\subsection*{12.}

\subsection*{14.}
$(B–C)DD^{–1} =0D^{–1}, (B–C)I=0, B–C=0, and B=C.$
\subsection*{15.}
$(ABC) C^{–1}B^{–1}A^{–1} = ABCC^{–1}B^{–1}A^{–1} = ABIB^{–1}A^{–1} = ABB^{–1}A^{–1} = AIA^{–1} = AA^{–1} = I$
\subsection*{18.}
$P^{–1}A = P^{–1}PBP^{–1}, \ P^{–1}A = IBP^{–1}, \ P^{–1}A = BP^{–1}$


\end{document}